alternative phrasing for em

Examples/HHS_Elgamal.lean
@@ -32,6 +32,19 @@ and the secret key is their vectorization in `G`. Signatures are also a pair of 
     return c₂ / (sk +ᵥ c₁)
   __ := ExecutionMethod.default
 
+@[simps!] def elgamalAsymmEnc' (G P : Type) [SelectableType G] [SelectableType P]
+    [AddGroup G] [Group P] [AddTorsor G P] : AsymmEncAlg' ProbComp
+    (M := P) (PK := P × P) (SK := G) (C := P × P) where
+  keygen := do
+    let x₀ ←$ᵗ P; let sk ←$ᵗ G
+    return ((x₀, sk +ᵥ x₀), sk)
+  encrypt := fun (x₀, pk) msg => do
+    let g ←$ᵗ G
+    return (g +ᵥ x₀, msg * (g +ᵥ pk))
+  decrypt := fun sk (c₁, c₂) => do
+    return c₂ / (sk +ᵥ c₁)
+  __ := ExecutionMethod.default
+
 namespace elgamalAsymmEnc
 
 variable {G P : Type} [SelectableType G] [SelectableType P]
@@ -46,6 +59,11 @@ variable {G P : Type} [SelectableType G] [SelectableType P]
 theorem Correct [DecidableEq P] : (elgamalAsymmEnc G P).PerfectlyCorrect := by
   have : ∀ (msg x : P) (g₁ g₂ : G), msg * (g₂ +ᵥ (g₁ +ᵥ x)) / (g₁ +ᵥ (g₂ +ᵥ x)) = msg :=
     fun m x g₁ g₂ => by rw [vadd_comm g₁ g₂ x, mul_div_cancel_right]
-  simp [this] -- Need to pass in one helper lemma to get the proof to go through.
+  simp [this]
+
+theorem Correct' [DecidableEq P] : AsymmEncAlg.PerfectlyCorrect' (elgamalAsymmEnc' G P) := by
+  have : ∀ (msg x : P) (g₁ g₂ : G), msg * (g₂ +ᵥ (g₁ +ᵥ x)) / (g₁ +ᵥ (g₂ +ᵥ x)) = msg :=
+    fun m x g₁ g₂ => by rw [vadd_comm g₁ g₂ x, mul_div_cancel_right]
+  simp [this, AsymmEncAlg.PerfectlyCorrect', AsymmEncAlg.CorrectExp']
 
 end elgamalAsymmEnc
